continue ...

srv.v
@@ -4,8 +4,7 @@ From iris.heap_lang Require Export lang.
 From iris.heap_lang Require Import proofmode notation.
 From iris.heap_lang.lib Require Import spin_lock.
 From iris.algebra Require Import upred frac agree excl dec_agree upred_big_op gset gmap.
-From iris.tests Require Import atomic treiber_stack.
-From flatcomb Require Import misc.
+From iris.tests Require Import misc atomic treiber_stack.
 
 Definition doOp (f: val) : val :=
   λ: "p",
@@ -19,14 +18,13 @@ Definition loop (f: val): val :=
     match: !"p" with
       InjL "_" =>
         if: try_acquire "lk"
-          then iter' (!"s") (doOp f);;
+          then iter (!"s") (doOp f);;
                release "lk";;
                "loop" "p" "s" "lk"
           else "loop" "p" "s" "lk"
     | InjR "r" => "r"
     end.
 
-(* Naive implementation *)
 Definition install : val :=
   λ: "x" "s",
      let: "p" := ref (InjL "x") in
@@ -44,16 +42,17 @@ Definition flat (f: val) : val :=
 Global Opaque doOp install loop flat.
 
 Definition srvR := prodR fracR (dec_agreeR val).
-Definition tokR := evmapR loc (gname * gname * gname * gname).
+Definition toks : Type := gname * gname * gname * gname.
+Definition tokmR := evmapR loc toks.
 Definition srvmR := evmapR loc val.
 Class srvG Σ := SrvG {
   srv_G :> inG Σ srvR;
-  tok_G :> inG Σ (authR tokR);
+  tok_G :> inG Σ (authR tokmR);
 }.
 
 Definition srvΣ : gFunctors :=
   #[ GFunctor (constRF srvR);
-     GFunctor (constRF (authR tokR))
+     GFunctor (constRF (authR tokmR))
    ].
 
 Instance subG_srvΣ {Σ} : subG srvΣ Σ → srvG Σ.
@@ -61,38 +60,38 @@ Proof. intros [?%subG_inG [?%subG_inG _]%subG_inv]%subG_inv. split; apply _. Qed
 
 Section proof.
   Context `{!heapG Σ, !lockG Σ, !evidenceG loc val Σ, !srvG Σ} (N : namespace).
+  Context (Q: val → val → Prop).
+  
+  (* p slot invariant *)
+  Definition p_inv (γm γ2: gname) (v: val) :=
+    (∃ (γx γ1 γ3 γ4: gname) (p : loc) (q: Qp),
+       v = #p ★ own γm (◯ ({[ p := (q, DecAgree (γx, γ1, γ3, γ4)) ]} : tokmR)) ★
+       ((* INIT *)
+        (∃ y: val, p ↦{1/2} InjRV y ★ own γ1 (Excl ()) ★ own γ3 (Excl ()))∨
+        (* INSTALLED *)
+        (∃ x: val, p ↦{1/2} InjLV x ★ own γx ((1/2)%Qp, DecAgree x) ★ own γ1 (Excl ()) ★ own γ4 (Excl ())) ∨
+        (* RECEIVED *)
+        (∃ x: val, p ↦{1/2} InjLV x ★ own γx ((1/2/2)%Qp, DecAgree x) ★ own γ2 (Excl ()) ★ own γ4 (Excl ())) ∨
+        (* FINISHED *)
+        (∃ x y: val, p ↦{1/2} InjRV y ★ own γx ((1/2)%Qp, DecAgree x) ★ ■ Q x y ★ own γ1 (Excl ()) ★ own γ4 (Excl ()))))%I.
 
-  Definition p_inv
-             (γm γx γ1 γ2 γ3 γ4: gname)
-             (Q: val → val → Prop)
-             (v: val): iProp Σ :=
-    (∃ (p : loc) (q: Qp), v = #p ★ own γm (◯ ({[ p := (q, DecAgree (γx, γ1, γ3, γ4)) ]} : tokR)) ★
-     ((∃ (y: val), p ↦{1/2} InjRV y ★ own γ1 (Excl ()) ★ own γ3 (Excl ())) ∨
-      (∃ (x: val), p ↦{1/2} InjLV x ★ own γx ((1/2)%Qp, DecAgree x) ★ own γ1 (Excl ()) ★ own γ4 (Excl ())) ∨
-      (∃ (x: val), p ↦{1/2} InjLV x ★ own γx ((1/2/2)%Qp, DecAgree x) ★ own γ2 (Excl ()) ★ own γ4 (Excl ())) ∨
-      (∃ (x y: val), p ↦{1/2} InjRV y ★ own γx ((1/2)%Qp, DecAgree x) ★ ■ Q x y ★ own γ1 (Excl ()) ★ own γ4 (Excl ()))))%I.
+  Definition srv_stack_inv (γs γm γ2: gname) (s: loc) := (∃ xs, is_stack' (p_inv γm γ2) γs xs s)%I.
 
-  Definition p_inv_R γm γ2 Q v : iProp Σ :=
-    (∃ γx γ1 γ3 γ4: gname, p_inv γm γx γ1 γ2 γ3 γ4 Q v)%I.
-
-  Definition srv_stack_inv (γ γm γ2: gname) (s: loc) (Q: val → val → Prop) : iProp Σ :=
-    (∃ xs, is_stack' (p_inv_R γm γ2 Q) xs s γ)%I.
-
-  Definition srv_m_inv γm := (∃ m : tokR, own γm (● m) ★ [★ map] p ↦ _ ∈ m, ∃ v, p ↦{1/2} v)%I.
+  Definition srv_tokm_inv γm := (∃ m : tokmR, own γm (● m) ★ [★ map] p ↦ _ ∈ m, ∃ v, p ↦{1/2} v)%I.
 
   Lemma install_push_spec
-        (Φ: val → iProp Σ) (Q: val → val → Prop)
-        (p: loc) (γ γm γx γ1 γ2 γ3 γ4: gname)
+        (Φ: val → iProp Σ)
+        (p: loc) (γs γm γx γ1 γ2 γ3 γ4: gname)
         (s: loc) (x: val) :
     heapN ⊥ N →
-    heap_ctx ★ inv N (srv_stack_inv γ γm γ2 s Q ★ srv_m_inv γm) ★ own γx ((1/2)%Qp, DecAgree x) ★
+    heap_ctx ★ inv N (srv_stack_inv γs γm γ2 s ★ srv_tokm_inv γm) ★ own γx ((1/2)%Qp, DecAgree x) ★
     own γm (◯ ({[ p := ((1 / 2)%Qp, DecAgree (γx, γ1, γ3, γ4)) ]})) ★
-    p ↦{1/2} InjLV x ★ own γ1 (Excl ()) ★ own γ4 (Excl ()) ★ ((∃ (hd : loc) (q : Qp), ev γ hd q #p) -★ Φ #())
+    p ↦{1/2} InjLV x ★ own γ1 (Excl ()) ★ own γ4 (Excl ()) ★ ((∃ hd, ev γs hd #p) -★ Φ #())
     ⊢ WP push #s #p {{ Φ }}.
   Proof.
     iIntros (HN) "(#Hh & #? & Hx & Hpm & Hp & Ho1 & Ho2 & HΦ)".
     rewrite /srv_stack_inv.
-    iDestruct (push_spec N (p_inv_R γm γ2 Q) (fun v => (∃ (hd : loc) (q : Qp), ev γ hd q #p) ★ v = #())%I
+    iDestruct (push_spec N (p_inv γm γ2) (fun v => (∃ hd, ev γs hd #p) ★ v = #())%I
                with "[-HΦ]") as "Hpush"=>//.
     - iFrame "Hh". iSplitL "Hx Hp Hpm Ho1 Ho2"; last eauto.
       iExists γx, γ1, γ3, γ4. iExists p, (1/2)%Qp. iSplit=>//. iFrame "Hpm".
@@ -105,13 +104,13 @@ Section proof.
   Qed.
 
   Lemma install_spec
-        (Φ: val → iProp Σ) (Q: val → val → Prop)
-        (x: val) (γ2 γm γ: gname) (s: loc):
+        (Φ: val → iProp Σ)
+        (x: val) (γs γm γ2: gname) (s: loc):
     heapN ⊥ N →
-    heap_ctx ★ inv N (srv_stack_inv γ γm γ2 s Q ★ srv_m_inv γm) ★ 
-    (∀ (p: loc) (γx γ1 γ2 γ3 γ4: gname),
+    heap_ctx ★ inv N (srv_stack_inv γs γm γ2 s ★ srv_tokm_inv γm) ★
+    (∀ (p: loc) (γx γ1 γ3 γ4: gname),
        own γ3 (Excl ()) -★ own γm (◯ {[ p := ((1 / 2)%Qp, DecAgree (γx, γ1, γ3, γ4)) ]}) -★
-       own γx ((1/2)%Qp, DecAgree x) -★ (∃ (hd : loc) (q : Qp), ev γ hd q #p) -★ Φ #p)
+       own γx ((1/2)%Qp, DecAgree x) -★ (∃ hd, ev γs hd #p) -★ Φ #p)
     ⊢ WP install x #s {{ Φ }}.
   Proof.
     iIntros (HN) "(#Hh & #? & HΦ)".
@@ -125,7 +124,7 @@ Section proof.
     iDestruct "Hm" as (m) "[Hm HRm]".
     destruct (m !! p) eqn:Heqn.
     - (* old name *)
-      iDestruct (split_mapk m with "[HRm]") as "[Hp HRm]"=>//.
+      iDestruct (big_sepM_delete (fun p _ => ∃ v : val, p ↦{1 / 2} v)%I m with "HRm") as "[Hp HRm]"=>//.
       iDestruct "Hp" as (?) "Hp". iExFalso. iApply bogus_heap; last by iFrame "Hh Hl Hp". auto.
     - (* fresh name *)
       iAssert (|=r=> own γm (● ({[p := (1%Qp, DecAgree (γx, γ1, γ3, γ4))]} ⋅ m) ⋅
@@ -134,7 +133,7 @@ Section proof.
         apply auth_update_no_frag. apply alloc_unit_singleton_local_update=>//. }
       iDestruct "Hl" as "[Hl1 Hl2]".
       iVs ("Hclose" with "[HRm Hm1 Hl1 Hrs]").
-      + iNext. iFrame. rewrite /srv_m_inv.  iExists ({[p := (1%Qp, DecAgree (γx, γ1, γ3, γ4))]} ⋅ m).
+      + iNext. iFrame. iExists ({[p := (1%Qp, DecAgree (γx, γ1, γ3, γ4))]} ⋅ m).
         iFrame.
         replace ({[p := (1%Qp, DecAgree (γx, γ1, γ3, γ4))]} ⋅ m) with
                 (<[p := (1%Qp, DecAgree (γx, γ1, γ3, γ4))]> m); last by apply insert_singleton_op.
@@ -151,139 +150,75 @@ Section proof.
         iApply install_push_spec=>//.
         iFrame "#". iFrame "Hx1 Hfrag1 Hl2 Ho1 Ho4".
         iIntros "Hev". wp_seq. iVsIntro.
-        iSpecialize ("HΦ" $! p γx γ1 γ2 γ3 γ4 with "[-Hx2 Hfrag2 Hev]")=>//.
+        iSpecialize ("HΦ" $! p γx γ1 γ3 γ4 with "[-Hx2 Hfrag2 Hev]")=>//.
         by iApply ("HΦ" with "Hfrag2 Hx2").
   Qed.
 
-  Lemma access x xs m Q (γ γm γ2: gname):
+  Lemma access (γ γm γ2: gname) x xs m :
     ∀ hd: loc,
     heapN ⊥ N → x ∈ xs  →
-    heap_ctx ★ ([★ map] _↦v ∈ m, ∃ v' : val,
-                                   v = (1%Qp, DecAgree v') ★ p_inv_R γm γ2 Q v') ★ own γ (● m) ★
+    heap_ctx ★ ([★ map] hd↦v ∈ m, perR (p_inv γm γ2) hd v) ★ own γ (● m) ★
     is_list' γ hd xs
-    ⊢ ∃ hd', (([★ map] _↦v ∈ delete hd' m, ∃ v' : val,
-                                           v = (1%Qp, DecAgree v') ★ p_inv_R γm γ2 Q v') ★
-         ∃ v, v = (1%Qp, DecAgree x) ★ p_inv_R γm γ2 Q x ★ m !! hd' = Some v) ★ own γ (● m).
+    ⊢ ∃ hd' v', ([★ map] hd↦v ∈ delete hd' m, perR (p_inv γm γ2) hd v) ★
+                perR' (p_inv γm γ2) hd' v' x ★ m !! hd' = Some v' ★ own γ (● m).
   Proof.
     induction xs as [|x' xs' IHxs'].
     - iIntros (? _ Habsurd). inversion Habsurd.
     - destruct (decide (x = x')) as [->|Hneq].
       + iIntros (hd HN _) "(#Hh & HR & Hom & Hxs)".
-        simpl. iDestruct "Hxs" as (hd' q p) "[Hhd [Hev Hxs']]".
+        simpl. iDestruct "Hxs" as (hd' q) "[Hhd [Hev Hxs']]".
         rewrite /ev. destruct (m !! hd) eqn:Heqn.
-        * iDestruct (split_mapv m with "[HR]") as "[Hp HRm]"=>//.
-          iDestruct "Hp" as (v') "[% ?]".
+        * iDestruct (big_sepM_delete (perR (p_inv γm γ2)) m with "HR") as "[Hp HRm]"=>//.
+          iDestruct "Hp" as (v') "[% [? ?]]".
           subst.
           destruct (decide (x' = v')) as [->|Hneq].
-          { iFrame. eauto. }
+          { iFrame. iExists hd. iFrame. iExists (1%Qp, DecAgree v'). iSplitL; auto. }
           { iExFalso.
-            iCombine "Hom" "Hev" as "Hauth".
-            iDestruct (own_valid γ (● m ⋅ ◯ {[hd := (p, DecAgree x')]}) with "[Hauth]") as %H=>//.
-            iPureIntro.
-            apply auth_valid_discrete_2 in H as [[af Compose%leibniz_equiv_iff] Valid].
-            eapply map_agree=>//. }
+            iDestruct "Hev" as (?) "Hev".  iCombine "Hom" "Hev" as "Hauth".
+            iDestruct (own_valid γ (● m ⋅ ◯ {[hd := (_, DecAgree x')]}) with "[Hauth]") as %Hvalid=>//.
+            iPureIntro. apply auth_valid_discrete_2 in Hvalid as [[af Compose%leibniz_equiv_iff] Valid].
+            apply Hneq. eapply (map_agree_eq _ _ m)=>//. }
         * iExFalso.
-          iCombine "Hom" "Hev" as "Hauth".
-          iDestruct (own_valid γ (● m ⋅ ◯ {[hd := (p, DecAgree x')]}) with "[Hauth]") as %H=>//.
-          iPureIntro.
-          apply auth_valid_discrete_2 in H as [[af Compose%leibniz_equiv_iff] Valid].
-          eapply map_agree_none=>//. rewrite Compose in Heqn. exact Heqn.
-      + iIntros (hd HN ?). 
+          iDestruct "Hev" as (?) "Hev".  iCombine "Hom" "Hev" as "Hauth".
+          iDestruct (own_valid γ (● m ⋅ ◯ {[hd := (_, DecAgree x')]}) with "[Hauth]") as %Hvalid=>//.
+          iPureIntro. apply auth_valid_discrete_2 in Hvalid as [[af Compose%leibniz_equiv_iff] Valid].
+          eapply (map_agree_none _ _ m)=>//.
+      + iIntros (hd HN ?).
         assert (x ∈ xs').
         { set_solver. }
         iIntros "(#Hh & HRs & Hom & Hxs')".
-        simpl. iDestruct "Hxs'" as (hd' q p) "[Hhd [Hev Hxs']]".
-        iApply IHxs'=>//.
+        simpl. iDestruct "Hxs'" as (hd' q) "[Hhd [Hev Hxs']]".
+        iDestruct (IHxs' hd' with "[HRs Hxs' Hom]") as "?"=>//.
         iFrame "#". iFrame.
   Qed.
 
-  Lemma map_agree_none' {A: cmraT} m m' (hd: loc) (q: A) (x: gname * gname * gname * gname):
-    m !! hd = None → m = {[hd := (q, DecAgree x)]} ⋅ m' → False.
-  Proof.
-    intros H1 H2. subst. rewrite lookup_op lookup_singleton in H1.
-    destruct (m' !! hd)=>//.
-  Qed.
-
-  Lemma m_frag_agree' γm p q1 q2 (γs1 γs2: gname * gname * gname * gname):
-    own γm (◯ {[p := (q1, DecAgree γs1)]}) ★
-    own γm (◯ {[p := (q2, DecAgree γs2)]})
-    ⊢ |=r=> own γm (◯ {[p := ((q1 + q2)%Qp, DecAgree γs1)]}) ★ (γs1 = γs2).
-  Proof.
-    iIntros "[Ho Ho']".
-    destruct (decide (γs1 = γs2)) as [->|Hneq].
-    - iSplitL=>//.
-      iCombine "Ho" "Ho'" as "Ho".
-      iDestruct (own_update with "Ho") as "?"; last by iAssumption.
-      rewrite <-(@auth_frag_op tokR {[p := (q1, DecAgree γs2)]} {[p := (q2, DecAgree γs2)]}).
-      by rewrite op_singleton pair_op frac_op' dec_agree_idemp.
-    - iCombine "Ho" "Ho'" as "Ho".
-      iDestruct (own_valid with "Ho") as %Hvalid.
-      exfalso. rewrite <-(@auth_frag_op tokR) in Hvalid.
-      rewrite op_singleton in Hvalid.
-      apply auth_valid_discrete in Hvalid. simpl in Hvalid.
-      apply singleton_valid in Hvalid.
-      destruct Hvalid as [_ Hvalid].
-      apply dec_agree_op_inv in Hvalid. inversion Hvalid. subst. auto.
-  Qed.
-
-    Lemma m_frag_agree γm q1 q2 (γs1 γs2: val):
-    own γm (q1, DecAgree γs1) ★ own γm (q2, DecAgree γs2)
-    ⊢ |=r=> own γm ((q1 + q2)%Qp, DecAgree γs1) ★ (γs1 = γs2).
-  Proof.
-    iIntros "[Ho Ho']".
-    destruct (decide (γs1 = γs2)) as [->|Hneq].
-    - iSplitL=>//.
-      iCombine "Ho" "Ho'" as "Ho".
-      iDestruct (own_update with "Ho") as "?"; last by iAssumption.
-      by rewrite pair_op frac_op' dec_agree_idemp.
-    - iCombine "Ho" "Ho'" as "Ho".
-      iDestruct (own_valid with "Ho") as %Hvalid.
-      exfalso. destruct Hvalid as [_ Hvalid].
-      simpl in Hvalid. apply dec_agree_op_inv in Hvalid. inversion Hvalid. subst. auto.
-  Qed.
-
-  Lemma in_m (m: srvmR) k q q' (a b: val) γ:
-    m !! k = Some (q, DecAgree a) →
-    own γ (● m) ★ own γ (◯ {[ k := (q', DecAgree b)]})
-    ⊢ own γ (● m) ★ own γ (◯ {[ k := (q', DecAgree a)]}) ★ a = b.
-  Proof.
-    iIntros (H) "[HFull HFrag]".
-    destruct (decide (a = b)).
-    - subst. by iFrame.
-    - iCombine "HFull" "HFrag" as "Hauth".
-      iDestruct (own_valid γ (● m ⋅ ◯ {[k := (q', DecAgree b)]}) with "[Hauth]") as %Hvalid=>//. 
-      exfalso. apply auth_valid_discrete_2 in Hvalid as [[af Compose%leibniz_equiv_iff] Valid].
-      eapply (map_agree m af)=>//. rewrite Compose in H. done.
-  Qed.
-
-  Lemma loop_iter_list_spec Φ (f: val) (s hd: loc) Q (γ γm γ2: gname) xs:
+  Lemma loop_iter_list_spec Φ (f: val) (s hd: loc) (γs γm γ2: gname) xs:
     heapN ⊥ N → (∀ x:val, True ⊢ WP f x {{ v, ■ Q x v }}) →
-    heap_ctx ★ inv N (srv_stack_inv γ γm γ2 s Q ★ srv_m_inv γm) ★ own γ2 (Excl ()) ★
-    is_list' γ hd xs ★ (own γ2 (Excl ()) -★ Φ #())
-    ⊢ WP iter' #hd (doOp f) {{ Φ }}.
+    heap_ctx ★ inv N (srv_stack_inv γs γm γ2 s ★ srv_tokm_inv γm) ★ own γ2 (Excl ()) ★
+    is_list' γs hd xs ★ (own γ2 (Excl ()) -★ Φ #())
+    ⊢ WP iter #hd (doOp f) {{ Φ }}.
   Proof.
     iIntros (HN Hf) "(#? & #? & Ho2 & Hlist' & HΦ)".
     iApply pvs_wp.
     iDestruct (dup_is_list' with "[Hlist']") as "==>[Hl1 Hl2]"; first by iFrame.
     iDestruct (dup_is_list' with "[Hl2]") as "==>[Hl2 Hl3]"; first by iFrame.
     iVsIntro.
-    iDestruct (iter'_spec _ (p_inv_R γm γ2 Q) (fun v => v = #() ★ own γ2 (Excl ()))%I γ s (is_list' γ hd xs ★ own γ2 (Excl ()))%I (srv_m_inv γm) xs hd
-                          (doOp f) (doOp f)
-              with "[-Hl1 HΦ]") as "Hiter'"=>//.
+    iDestruct (iter_spec _ (p_inv γm γ2) (fun v => v = #() ★ own γ2 (Excl ()))%I γs s (is_list' γs hd xs ★ own γ2 (Excl ()))%I (srv_tokm_inv γm) xs hd (doOp f) (doOp f)
+              with "[-Hl1 HΦ]") as "Hiter"=>//.
     - rewrite /f_spec. 
       iIntros (Φ' p _ Hin) "(#Hh & #? & (Hls & Ho2) & HΦ')".
       wp_let. wp_bind (! _)%E. iInv N as ">[Hs Hm]" "Hclose".
       iDestruct "Hs" as (xs' hd') "[Hhd [Hxs HRs]]".
       iDestruct (dup_is_list' with "[Hls]") as "==>[Hls1 Hls2]"; first by iFrame.
       iDestruct "HRs" as (m) "[Hom HRs]".
-      iDestruct (access with "[Hom HRs Hls1]") as (hd'') "[[Hops Hop2] Hom']"=>//; first by iFrame.
-      iDestruct "Hop2" as ([q x]) "(% & H & %)".
+      iDestruct (access with "[Hom HRs Hls1]") as (hd'' [q x]) "[Hrest [Hhd'' [% Hom]]]"=>//; first by iFrame.
+      iDestruct "Hhd''" as "(% & H & Hphd)". inversion H0. subst.
       iDestruct "H" as (γx γ1 γ3 γ4 p'' q'') "[% [Hop [Hp | [Hp | [Hp | Hp]]]]]"; subst.
       + iDestruct "Hp" as (x') "(Hp & Ho1 & Ho3)".
         wp_load. iVs ("Hclose" with "[-HΦ' Ho2 Hls2]").
         { iNext. iFrame. iExists xs', hd'.
           iFrame "Hhd Hxs". iExists m.
-          iFrame "Hom'". iDestruct (merge_mapv m with "[Hop Hops Hp Ho1 Ho3]") as "?"=>//.
+          iFrame "Hom". iDestruct (big_sepM_delete _ m with "[Hrest Hphd Hop Hp Ho1 Ho3]") as "?"=>//.
           iFrame. iExists #p''. iSplitR; first auto. iExists γx, γ1, γ3, γ4, p'', q''.
           iSplitR; auto. iFrame. iLeft. iExists x'. iFrame. }
         iVsIntro. wp_match. iApply "HΦ'". iFrame.
@@ -303,8 +238,8 @@ Section proof.
         iVs ("Hclose" with "[-Hls2 Ho1 Hx2 Hop2 HΦ']").
         { iNext. iFrame. iExists xs', hd'.
           iFrame "Hhd Hxs". iExists m.
-          iFrame "Hom'". iDestruct (merge_mapv m with "[Hop1 Hops Hp Hx1 Ho2 Ho4]") as "?"=>//.
-          simpl. iFrame. iExists #p''.  iSplitR; auto.
+          iFrame "Hom". iDestruct (big_sepM_delete _ m with "[-]") as "?"=>//.
+          simpl. iFrame. iExists #p''.  iSplitR; auto. rewrite /allocated.
           iExists γx, γ1, γ3, γ4, p'', (q''/2)%Qp. iSplitR; auto.
           iFrame. iRight. iRight. iLeft. iExists x'. iFrame. }
         iVsIntro. wp_match.
@@ -314,8 +249,8 @@ Section proof.
         iDestruct "Hs" as (xs'' hd''') "[Hhd [Hxs HRs]]".
         iDestruct "HRs" as (m') "[Hom HRs]".
         iDestruct (dup_is_list' with "[Hls2]") as "==>[Hls2 Hls3]"; first by iFrame.
-        iDestruct (access with "[Hom HRs Hls2]") as (hd'''') "[[Hops Hop3] Hom']"=>//; first by iFrame.
-        iDestruct "Hop3" as ([q''' x''']) "(% & H & %)".
+        iDestruct (access with "[Hom HRs Hls2]") as (hd'''' [q x]) "[Hrest [Hhd'' [% Hom]]]"=>//; first by iFrame.
+        iDestruct "Hhd''" as "(% & H & Hphd)". inversion H3. subst.
         iDestruct "H" as (γx' γ1' γ3' γ4' p'''' q'''') "[% [Hop Hps]]".
         inversion H4.
         destruct (decide (γ1 = γ1' ∧ γx = γx' ∧ γ3 = γ3' ∧ γ4 = γ4')) as [[? [? [? ?]]]|Hneq].
@@ -332,30 +267,27 @@ Section proof.
             iDestruct "Hm" as (m2) "[Hom2 HRm]".
             destruct (m2 !! p'''') eqn:Heqn.
             { 
-              iDestruct (split_mapk m2 with "[HRm]") as "[HRk HRm]"=>//.
+              iDestruct (big_sepM_delete _ m2 with "HRm") as "[HRk HRm]"=>//.
               iDestruct "HRk" as (?) "HRk".
               iDestruct (heap_mapsto_op_1 with "[HRk Hp]") as "[% Hp]"; first by iFrame.
               rewrite Qp_div_2. wp_store.
               (* now close the invariant *)
               iDestruct (m_frag_agree with "[Hx Hx2]") as "==>[Hx %]"; first iFrame.
-              subst.
-              rewrite Qp_div_2.
-              iVs ("Hclose" with "[-HΦ' Ho2 Hls3]").
-              { iNext.
-                iDestruct "Hp" as "[Hp1 Hp2]".
-                iAssert (srv_m_inv γm) with "[Hp1 HRm Hom2]" as "HRm".
-                { iExists m2. iFrame. iApply (merge_mapk m2)=>//.
+              subst. rewrite Qp_div_2. iVs ("Hclose" with "[-HΦ' Ho2 Hls3]").
+              { iNext. iDestruct "Hp" as "[Hp1 Hp2]".
+                iAssert (srv_tokm_inv γm) with "[Hp1 HRm Hom2]" as "HRm".
+                { iExists m2. iFrame. iApply (big_sepM_delete _ m2)=>//.
                   iFrame. eauto. }
                 iFrame. iExists xs''. iFrame. iExists hd'''. iFrame.
                 iExists m'. iFrame.
-                iDestruct (merge_mapv m' with "[-]") as "?"=>//.
-                { simpl. iFrame. rewrite H2. iExists #p''''.
+                iDestruct (big_sepM_delete _ m' with "[-]") as "?"=>//.
+                { simpl. iFrame. iExists #p''''.
                   iSplitR; first auto. iExists γx', γ1', γ3', γ4'.
                   rewrite /p_inv. iExists p'''', q''''.
                   iSplitR; first auto. iFrame. iRight. iRight.
-                  iRight. iExists x5, v. iFrame. done. }
+                  iRight. iExists x5, v. by iFrame. }
               }
-              iApply "HΦ'". iFrame. 
+              iApply "HΦ'". iFrame.
             }
             { iExFalso.
               iCombine "Hom2" "Hop2" as "Hauth".
@@ -364,12 +296,13 @@ Section proof.
                     := ((q'' / 2)%Qp, DecAgree (γx', γ1', γ3', γ4'))]}) with "[Hauth]") as %Hvalid=>//.
               iPureIntro.
               apply auth_valid_discrete_2 in Hvalid as [[af Compose%leibniz_equiv_iff] Valid].
-              eapply map_agree_none'=>//. }
+              eapply (map_agree_none _ _ m2)=>//.
+            }
           * iDestruct "Hp" as (? ?) "(_ & _ & _ & Ho1' & _)".
             iExFalso. iCombine "Ho1" "Ho1'" as "Ho1".
             by iDestruct (own_valid with "Ho1") as "%". }
-        { iDestruct (m_frag_agree' with "[Hop Hop2]") as "==>[Hop %]"; first iFrame.
-           inversion H5. subst. exfalso. apply Hneq. auto. }
+        { iDestruct (evmap_frag_agree with "[Hop Hop2]") as "==>[Hop %]"; first iFrame.
+          inversion H5. subst. exfalso. apply Hneq. auto. }
       + iDestruct "Hp" as (y) "(Hp & Hx & Ho2' & Ho4)".
         iExFalso. iCombine "Ho2" "Ho2'" as "Ho2".
         by iDestruct (own_valid with "Ho2") as "%".
@@ -377,22 +310,36 @@ Section proof.
         wp_load. iVs ("Hclose" with "[-HΦ' Ho2 Hls2]").
         { iNext. iFrame. iExists xs', hd'.
           iFrame "Hhd Hxs". iExists m.
-          iFrame "Hom'". iDestruct (merge_mapv m with "[Hop Hops Hp Ho1 Ho4]") as "?"=>//.
+          iFrame "Hom". iDestruct (big_sepM_delete _ m with "[Hop Hphd Hrest Hp Ho1 Ho4]") as "?"=>//.
           iFrame. iExists #p''. iSplitR; first auto. iExists γx, γ1, γ3, γ4, p'', q''.
           iSplitR; auto. iFrame. iRight. iRight. iRight. iExists x', y. iFrame. }
         iVsIntro. wp_match. iApply "HΦ'". iFrame.
     - apply to_of_val.
     - rewrite /srv_stack_inv. iFrame "#". iFrame. iIntros "[_ Ho2]". eauto.
-    - iApply wp_wand_r. iSplitL "Hiter'"; first done.
+    - iApply wp_wand_r. iSplitL "Hiter"; first done.
       iIntros (?) "[% Ho2]". subst. by iApply "HΦ".
   Qed.
-      
+
+  Lemma in_m γs (m: srvmR) k q q' (a b: val):
+    m !! k = Some (q, DecAgree b) →
+    own γs (● m) ★ own γs (◯ {[ k := (q', DecAgree a)]})
+    ⊢ own γs (● m) ★ own γs (◯ {[ k := (q', DecAgree a)]}) ★ a = b.
+  Proof.
+    iIntros (H) "[HFull HFrag]".
+    destruct (decide (a = b)) as [->|Hneq].
+    - by iFrame.
+    - iCombine "HFull" "HFrag" as "Hauth".
+      iDestruct (own_valid γs (● m ⋅ ◯ {[k := (q', DecAgree a)]}) with "[Hauth]") as %Hvalid=>//.
+      exfalso. apply auth_valid_discrete_2 in Hvalid as [[af Compose%leibniz_equiv_iff] Valid].
+      apply Hneq. eapply (map_agree_eq _ _ m); done.
+  Qed.
+
   Lemma loop_spec Φ (p s: loc) (lk: val) (f: val)
-        Q (γ2 γm γ γlk: gname) (γx γ1 γ3 γ4: gname):
+        (γs γ2 γm γlk: gname) (γx γ1 γ3 γ4: gname):
     heapN ⊥ N → (∀ x:val, True ⊢ WP f x {{ v, ■ Q x v }}) →
-    heap_ctx ★ inv N (srv_stack_inv γ γm γ2 s Q ★ srv_m_inv γm) ★ is_lock N γlk lk (own γ2 (Excl ())) ★
+    heap_ctx ★ inv N (srv_stack_inv γs γm γ2 s ★ srv_tokm_inv γm) ★ is_lock N γlk lk (own γ2 (Excl ())) ★
     own γ3 (Excl ()) ★ (∃ q: Qp, own γm (◯ {[ p := (q, DecAgree (γx, γ1, γ3, γ4)) ]})) ★
-    (∃ hd q, ev γ hd q #p) ★ (∀ x y,  own γx ((1 / 2)%Qp, DecAgree x) -★ ■ Q x y -★ Φ y)
+    (∃ hd, ev γs hd #p) ★ (∀ x y,  own γx ((1 / 2)%Qp, DecAgree x) -★ ■ Q x y -★ Φ y)
     ⊢ WP loop f #p #s lk {{ Φ }}.
   Proof.
     iIntros (HN Hf) "(#Hh & #? & #? & Ho3 & Hγs & Hev & HΦ)".
@@ -403,59 +350,69 @@ Section proof.
     iDestruct "HRs" as (m) "[Hom HRs]".
     iDestruct "Hev" as (hdp ?) "Hev".
     rewrite /ev. destruct (m !! hdp) eqn:Heqn.
-    - iDestruct (split_mapv m with "[HRs]") as "[Hp Hrs]"=>//.
-      iDestruct "Hp" as (?) "[% Hpr]"; subst.
+    - iDestruct (big_sepM_delete _ m with "HRs") as "[Hp Hrs]"=>//.
+      iDestruct "Hp" as (?) "[% [Hpr ?]]"; subst.
       iDestruct "Hpr" as (γx' γ1' γ3' γ4' p' q') "(% & Hp' & Hp)".
-      subst. iDestruct (in_m with "[Hom Hev]") as "(Hom & Hev & %)"=>//; first iFrame.
+      subst. iDestruct (in_m γs with "[Hom Hev]") as "(Hom & Hev & %)"=>//; first iFrame; eauto.
       inversion H0. subst.
-      iDestruct (m_frag_agree' with "[Hγs Hp']") as "==>[Hγs %]"; first iFrame.
+      iDestruct (evmap_frag_agree_split with "[Hγs Hp']") as "==>[Hγs2 [Hγs %]]"; first iFrame.
       inversion H1. subst.
       iDestruct "Hp" as "[Hp | [Hp | [ Hp | Hp]]]".
-      + (* trivial *) admit.
+      + iDestruct "Hp" as (?) "(_ & _ & Ho3')".
+        iExFalso. iCombine "Ho3" "Ho3'" as "Ho3".
+        by iDestruct (own_valid with "Ho3") as "%".
       + iDestruct "Hp" as (x) "(Hp & Hx & Ho1 & Ho4)".
         wp_load.
-        iVs ("Hclose" with "[-Hγs Ho3 HΦ Hev]"). (* Hev here should be a duplicated one *)
-        { iNext. iFrame. iExists xs, hd. iFrame. iExists m. iFrame. (* merge *) admit. }
-        iVsIntro. wp_match. (* we should close it as it is in this case *)
-        (* now, just reason like a server *)
-        wp_bind (try_acquire _). iApply try_acquire_spec.
-        iFrame "#". iSplit.
-        { (* acquired the lock *)
-          iIntros "Hlocked Ho2".
-          wp_if. wp_bind ((iter' _) _). wp_bind (! _)%E.
-          iInv N as ">[H Hm]" "Hclose".
-          iDestruct "H" as (xs' hd') "[Hs [Hxs HRs]]".
-          wp_load. iDestruct (dup_is_list' with "[Hxs]") as "==>[Hxs1 Hxs2]"; first by iFrame.
-          iVs ("Hclose" with "[Hs Hxs1 HRs Hm]").
-          { iNext. iFrame. iExists xs', hd'. by iFrame. }
-          iVsIntro. iApply loop_iter_list_spec=>//.
-          iFrame "#". iFrame. iIntros "Ho2".
-          wp_seq. wp_bind (release _). iApply release_spec.
-          iFrame "~ Hlocked Ho2". wp_seq.
-          iAssert ((∃ q0 : Qp,
-                      own γm (◯ {[p := (q0, DecAgree (γx, γ1, γ3, γ4))]})))%I with "[Hγs]" as "Hγs".
-          { eauto. }
-          iAssert (∃ (hd0 : loc) (q0 : Qp), own γ (◯ {[hd0 := (q0, DecAgree #p)]}))%I with "[Hev]" as "Hev".
-          { eauto. }
-          by iApply ("IH" with "Ho3 Hγs Hev"). }
-        {  wp_if.
-           iAssert ((∃ q0 : Qp,
-                        own γm (◯ {[p := (q0, DecAgree (γx, γ1, γ3, γ4))]})))%I with "[Hγs]" as "Hp'".
-            { eauto. }
-          iAssert (∃ (hd0 : loc) (q0 : Qp), own γ (◯ {[hd0 := (q0, DecAgree #p)]}))%I with "[Hev]" as "Hev".
-          { eauto. }
-            iApply ("IH" with "Ho3 Hp' Hev")=>//. }
-      + iDestruct "Hp" as (x) "(Hp & Hx & Ho2 & Ho4)".
-        wp_load.
-        iVs ("Hclose" with "[-Hγs Ho3 HΦ Hev]").
-        { iNext. iFrame. iExists xs, hd. iFrame. iExists m. iFrame. (* merge *) admit. }
+        iVs ("Hclose" with "[-Hγs2 Ho3 HΦ Hev]"). (* Hev here should be a duplicated one *)
+        { iNext. iFrame. iExists xs, hd. iFrame. iExists m. iFrame.
+          iDestruct (big_sepM_delete _ m with "[-]") as "?"=>//.
+          iFrame. iExists #p'. iSplitR; first auto. iExists γx, γ1, γ3, γ4, p', q.
+          iSplitR; first auto. iFrame.
+          iRight. iLeft. iExists x.
+          iFrame. } 
         iVsIntro. wp_match.
         (* now, just reason like a server *)
         wp_bind (try_acquire _). iApply try_acquire_spec.
         iFrame "#". iSplit.
         { (* acquired the lock *)
           iIntros "Hlocked Ho2".
-          wp_if. wp_bind ((iter' _) _). wp_bind (! _)%E.
+          wp_if. wp_bind ((iter _) _). wp_bind (! _)%E.
+          iInv N as ">[H Hm]" "Hclose".
+          iDestruct "H" as (xs' hd') "[Hs [Hxs HRs]]".
+          wp_load. iDestruct (dup_is_list' with "[Hxs]") as "==>[Hxs1 Hxs2]"; first by iFrame.
+          iVs ("Hclose" with "[Hs Hxs1 HRs Hm]").
+          { iNext. iFrame. iExists xs', hd'. by iFrame. }
+          iVsIntro. iApply loop_iter_list_spec=>//.
+          iFrame "#". iFrame. iIntros "Ho2".
+          wp_seq. wp_bind (release _). iApply release_spec.
+          iFrame "~ Hlocked Ho2". wp_seq.
+          iAssert ((∃ q0 : Qp, own γm (◯ {[p' := (q0, DecAgree (γx, γ1, γ3, γ4))]})))%I
+                  with "[Hγs2]" as "Hγs"; eauto.
+          iAssert (∃ (hd0 : loc) (q0 : Qp), own γs (◯ {[hd0 := (q0, DecAgree #p')]}))%I
+                  with "[Hev]" as "Hev"; eauto.
+          by iApply ("IH" with "Ho3 Hγs Hev"). }
+        {  wp_if.
+           iAssert (∃ q0 : Qp, own γm (◯ {[p' := (q0, DecAgree (γx, γ1, γ3, γ4))]}))%I
+                    with "[Hγs2]" as "Hp'"; eauto.
+           iAssert (∃ (hd0 : loc) (q0 : Qp), own γs (◯ {[hd0 := (q0, DecAgree #p')]}))%I
+                   with "[Hev]" as "Hev"; eauto.
+            iApply ("IH" with "Ho3 Hp' Hev")=>//. }
+      + iDestruct "Hp" as (x) "(Hp & Hx & Ho2 & Ho4)".
+        wp_load.
+        iVs ("Hclose" with "[-Hγs Ho3 HΦ Hev]").
+        { iNext. iFrame. iExists xs, hd. iFrame. iExists m. iFrame.
+          iDestruct (big_sepM_delete _ m with "[-]") as "?"=>//.
+          iFrame. iExists #p'. iSplitR; auto. iExists γx, γ1, γ3, γ4, p', q'.
+          iSplitR; first auto. iFrame. iFrame.
+          iRight. iRight. iLeft. iExists x. iFrame.
+        }
+        iVsIntro. wp_match.
+        (* now, just reason like a server *)
+        wp_bind (try_acquire _). iApply try_acquire_spec.
+        iFrame "#". iSplit.
+        { (* acquired the lock *)
+          iIntros "Hlocked Ho2".
+          wp_if. wp_bind ((iter _) _). wp_bind (! _)%E.
           iInv N as ">[H Hm]" "Hclose".
           iDestruct "H" as (xs' hd') "[Hs [Hxs HRs]]".
           wp_load. iDestruct (dup_is_list' with "[Hxs]") as "==>[Hxs1 Hxs2]"; first by iFrame.
@@ -466,49 +423,56 @@ Section proof.
           wp_seq. wp_bind (release _). iApply release_spec.
           iFrame "~ Hlocked Ho2". wp_seq.
           iAssert ((∃ q0 : Qp,
-                      own γm (◯ {[p := (q0, DecAgree (γx, γ1, γ3, γ4))]})))%I with "[Hγs]" as "Hγs".
+                      own γm (◯ {[p' := (q0, DecAgree (γx, γ1, γ3, γ4))]})))%I with "[Hγs]" as "Hγs".
           { eauto. }
-          iAssert (∃ (hd0 : loc) (q0 : Qp), own γ (◯ {[hd0 := (q0, DecAgree #p)]}))%I with "[Hev]" as "Hev".
+          iAssert (∃ (hd0 : loc) (q0 : Qp), own γs (◯ {[hd0 := (q0, DecAgree #p')]}))%I with "[Hev]" as "Hev".
           { eauto. }
             by iApply ("IH" with "Ho3 Hγs Hev"). }
         {  wp_if.
            iAssert ((∃ q0 : Qp,
-                       own γm (◯ {[p := (q0, DecAgree (γx, γ1, γ3, γ4))]})))%I with "[Hγs]" as "Hp'".
+                       own γm (◯ {[p' := (q0, DecAgree (γx, γ1, γ3, γ4))]})))%I with "[Hγs]" as "Hp'".
            { eauto. }
-           iAssert (∃ (hd0 : loc) (q0 : Qp), own γ (◯ {[hd0 := (q0, DecAgree #p)]}))%I with "[Hev]" as "Hev".
+           iAssert (∃ (hd0 : loc) (q0 : Qp), own γs (◯ {[hd0 := (q0, DecAgree #p')]}))%I with "[Hev]" as "Hev".
           { eauto. }
             iApply ("IH" with "Ho3 Hp' Hev")=>//. }
-            (* the #2 and #3 processing are identical *)
-      + iDestruct "Hp" as (x y) "(Hp & Hox & % & Ho1 & Ho4)".
-          wp_load.
-          iVs ("Hclose" with "[-Hγs Ho3 HΦ Hox]").
-          { iNext. iFrame. iExists xs, hd. iFrame. iExists m. iFrame. (* merge *) admit. }
-          iVsIntro. wp_match. by iApply ("HΦ" with "Hox").
-    - iExFalso. admit. (* this is the second hardest part *)
-  Admitted.
+      + iDestruct "Hp" as (x y) "(Hp & Hx & % & Ho1 & Ho4)".
+          wp_load. 
+          iVs ("Hclose" with "[-Hγs Ho4 HΦ Hx]").
+          { iNext. iFrame. iExists xs, hd. iFrame. iExists m. iFrame.
+            iDestruct (big_sepM_delete _ m with "[-]") as "?"=>//.
+            iFrame. iExists #p'. iSplitR; auto. iExists γx, γ1, γ3, γ4, p', q'.
+            iSplitR; first auto. iFrame. iFrame.
+            iLeft. iExists y. iFrame. }            
+          iVsIntro. wp_match. iApply ("HΦ" with "[-]").
+          iFrame. done.
+    - iExFalso.
+      iCombine "Hom" "Hev" as "Hauth".
+      iDestruct (own_valid γs (● m ⋅ ◯ {[hdp := (H, DecAgree #p)]}) with "[Hauth]") as %Hvalid=>//.
+      iPureIntro.
+      apply auth_valid_discrete_2 in Hvalid as [[af Compose%leibniz_equiv_iff] Valid].
+      eapply (map_agree_none _ _ m)=>//.
+  Qed.
 
-  Lemma flat_spec (f: val) Q:
+  Lemma flat_spec (f: val):
     heapN ⊥ N → (∀ x:val, True ⊢ WP f x {{ v, ■ Q x v }}) →
     heap_ctx ⊢ WP flat f #() {{ f', □ (∀ x: val, WP f' x {{ v, ■ Q x v }}) }}.
   Proof.
     iIntros (HN Hf) "#Hh".
     iVs (own_alloc (Excl ())) as (γ2) "Ho2"; first done.
-    iVs (own_alloc (● (∅: tokR) ⋅ ◯ ∅)) as (γm) "[Hm _]".
-    { by rewrite -auth_both_op. }
-    iAssert (srv_m_inv γm) with "[Hm]" as "Hm"; first eauto.
-    { rewrite /srv_m_inv. iExists ∅. iFrame. (* XXX: iApply big_sepM_empty. *)
-      by rewrite /uPred_big_sepM map_to_list_empty. }
+    iVs (own_alloc (● (∅: tokmR) ⋅ ◯ ∅)) as (γm) "[Hm _]"; first by rewrite -auth_both_op.
+    iAssert (srv_tokm_inv γm) with "[Hm]" as "Hm"; first eauto.
+    { iExists ∅. iFrame. by rewrite big_sepM_empty. }
     wp_seq. wp_bind (newlock _).
     iApply newlock_spec=>//.
     iFrame "Hh Ho2". iIntros (lk γlk) "#Hlk".
     wp_let. wp_bind (new_stack _).
-    iApply (new_stack_spec' _ (p_inv_R γm γ2 Q))=>//.
+    iApply (new_stack_spec' _ (p_inv γm γ2))=>//.
     iFrame "Hh Hm". iIntros (γ s) "#Hss".
     wp_let. iVsIntro. iAlways.
     iIntros (x). wp_let.
     wp_bind ((install _) _).
     iApply install_spec=>//.
-    iFrame "Hh Hss". iIntros (p γx γ1 _ γ3 γ4) "Hp3 Hpx Hx Hev".
+    iFrame "Hh Hss". iIntros (p γx γ1 γ3 γ4) "Hp3 Hpx Hx Hev".
     wp_let. iApply loop_spec=>//.
     iFrame "Hh Hss Hlk". iFrame.
     iSplitL "Hpx"; first eauto.
